<?xml version="1.0"?>
<rdf:RDF xmlns="https://raw.githubusercontent.com/TheWorldAvatar/ontovertopping/refs/heads/main/OntOvertopping.owl#"
     xml:base="https://raw.githubusercontent.com/TheWorldAvatar/ontovertopping/refs/heads/main/OntOvertopping.owl"
     xmlns:dc="http://purl.org/dc/elements/1.1/"
     xmlns:owl="http://www.w3.org/2002/07/owl#"
     xmlns:rdf="http://www.w3.org/1999/02/22-rdf-syntax-ns#"
     xmlns:xml="http://www.w3.org/XML/1998/namespace"
     xmlns:xsd="http://www.w3.org/2001/XMLSchema#"
     xmlns:rdfs="http://www.w3.org/2000/01/rdf-schema#"
     xmlns:terms="http://purl.org/dc/terms/"
     xmlns:OntOvertopping="https://raw.githubusercontent.com/TheWorldAvatar/ontovertopping/refs/heads/main/OntOvertopping.owl#">
    <owl:Ontology rdf:about="https://raw.githubusercontent.com/TheWorldAvatar/ontovertopping/refs/heads/main/OntOvertopping.owl">
        <dc:date>19 June 2025</dc:date>
        <terms:license>https://github.com/TheWorldAvatar/ontology/blob/main/LICENSE.txt</terms:license>
        <rdfs:comment>OntOvertopping is an ontology developed for representing wave conditions and overtopping discharge in coastal and port environments.</rdfs:comment>
        <owl:versionInfo>1</owl:versionInfo>
        <gitCommitHash>c0599beca8df55873a1ab061dee64e52c510c6a0</gitCommitHash>
    </owl:Ontology>
    


    <!-- 
    ///////////////////////////////////////////////////////////////////////////////////////
    //
    // Annotation properties
    //
    ///////////////////////////////////////////////////////////////////////////////////////
     -->


    


    <!-- http://purl.org/dc/elements/1.1/date -->


    <owl:AnnotationProperty rdf:about="http://purl.org/dc/elements/1.1/date"/>
    


    <!-- http://purl.org/dc/terms/license -->


    <owl:AnnotationProperty rdf:about="http://purl.org/dc/terms/license"/>
    


    <!-- https://raw.githubusercontent.com/TheWorldAvatar/ontovertopping/refs/heads/main/OntOvertopping.owl#gitCommitHash -->


    <owl:AnnotationProperty rdf:about="https://raw.githubusercontent.com/TheWorldAvatar/ontovertopping/refs/heads/main/OntOvertopping.owl#gitCommitHash"/>
    


    <!-- 
    ///////////////////////////////////////////////////////////////////////////////////////
    //
    // Object Properties
    //
    ///////////////////////////////////////////////////////////////////////////////////////
     -->


    


    <!-- http://www.ontology-of-units-of-measure.org/resource/om-2/hasUnit -->


    <owl:ObjectProperty rdf:about="http://www.ontology-of-units-of-measure.org/resource/om-2/hasUnit">
        <rdfs:domain rdf:resource="http://www.ontology-of-units-of-measure.org/resource/om-2/Measure"/>
        <rdfs:range rdf:resource="http://www.ontology-of-units-of-measure.org/resource/om-2/Unit"/>
        <rdfs:comment>An object property referring to the unit associated with a measured value.</rdfs:comment>
        <rdfs:isDefinedBy rdf:resource="http://www.ontology-of-units-of-measure.org/resource/om-2"/>
        <rdfs:label>hasUnit</rdfs:label>
    </owl:ObjectProperty>
    


    <!-- http://www.ontology-of-units-of-measure.org/resource/om-2/hasValue -->


    <owl:ObjectProperty rdf:about="http://www.ontology-of-units-of-measure.org/resource/om-2/hasValue">
        <rdfs:domain rdf:resource="http://www.ontology-of-units-of-measure.org/resource/om-2/Quantity"/>
        <rdfs:range rdf:resource="http://www.ontology-of-units-of-measure.org/resource/om-2/Measure"/>
        <rdfs:comment>An object property referring to the measured value of a quantity.</rdfs:comment>
        <rdfs:label>hasValue</rdfs:label>
    </owl:ObjectProperty>
    


    <!-- https://raw.githubusercontent.com/TheWorldAvatar/ontovertopping/refs/heads/main/OntOvertopping.owl#attacks -->


    <owl:ObjectProperty rdf:about="https://raw.githubusercontent.com/TheWorldAvatar/ontovertopping/refs/heads/main/OntOvertopping.owl#attacks">
        <rdfs:domain rdf:resource="https://raw.githubusercontent.com/TheWorldAvatar/ontovertopping/refs/heads/main/OntOvertopping.owl#Wave"/>
        <rdfs:range rdf:resource="https://raw.githubusercontent.com/TheWorldAvatar/ontovertopping/refs/heads/main/OntOvertopping.owl#CoastalDefenceStructure"/>
        <rdfs:comment>Relates a wave to the CoastalDefenceStructure that it impacts or overtops.</rdfs:comment>
        <rdfs:isDefinedBy rdf:resource="https://raw.githubusercontent.com/TheWorldAvatar/ontovertopping/refs/heads/main/OntOvertopping.owl"/>
        <rdfs:label>attacks</rdfs:label>
    </owl:ObjectProperty>
    


    <!-- https://raw.githubusercontent.com/TheWorldAvatar/ontovertopping/refs/heads/main/OntOvertopping.owl#generates -->


    <owl:ObjectProperty rdf:about="https://raw.githubusercontent.com/TheWorldAvatar/ontovertopping/refs/heads/main/OntOvertopping.owl#generates">
        <rdfs:domain rdf:resource="https://raw.githubusercontent.com/TheWorldAvatar/ontovertopping/refs/heads/main/OntOvertopping.owl#OvertoppingForecastModel"/>
        <rdfs:range rdf:resource="https://raw.githubusercontent.com/TheWorldAvatar/ontovertopping/refs/heads/main/OntOvertopping.owl#OvertoppingForecast"/>
        <rdfs:comment>An object property that links a model responsible for predicting overtopping events to the overtopping forecast it produces.</rdfs:comment>
        <rdfs:isDefinedBy rdf:resource="https://raw.githubusercontent.com/TheWorldAvatar/ontovertopping/refs/heads/main/OntOvertopping.owl"/>
        <rdfs:label>generates</rdfs:label>
    </owl:ObjectProperty>
    


    <!-- https://raw.githubusercontent.com/TheWorldAvatar/ontovertopping/refs/heads/main/OntOvertopping.owl#hasAttackAngle -->


    <owl:ObjectProperty rdf:about="https://raw.githubusercontent.com/TheWorldAvatar/ontovertopping/refs/heads/main/OntOvertopping.owl#hasAttackAngle">
        <rdfs:domain rdf:resource="https://raw.githubusercontent.com/TheWorldAvatar/ontovertopping/refs/heads/main/OntOvertopping.owl#Wave"/>
        <rdfs:range rdf:resource="https://raw.githubusercontent.com/TheWorldAvatar/ontovertopping/refs/heads/main/OntOvertopping.owl#AngleOfWaveAttack"/>
        <rdfs:comment>Relates a wave to the AngleOfWaveAttack, representing the angle it forms with the CrestWall.</rdfs:comment>
        <rdfs:isDefinedBy rdf:resource="https://raw.githubusercontent.com/TheWorldAvatar/ontovertopping/refs/heads/main/OntOvertopping.owl"/>
        <rdfs:label>hasAttackAngle</rdfs:label>
    </owl:ObjectProperty>
    


    <!-- https://raw.githubusercontent.com/TheWorldAvatar/ontovertopping/refs/heads/main/OntOvertopping.owl#hasInputParameter -->


    <owl:ObjectProperty rdf:about="https://raw.githubusercontent.com/TheWorldAvatar/ontovertopping/refs/heads/main/OntOvertopping.owl#hasInputParameter">
        <rdfs:domain rdf:resource="https://raw.githubusercontent.com/TheWorldAvatar/ontovertopping/refs/heads/main/OntOvertopping.owl#OvertoppingForecastModel"/>
        <rdfs:range rdf:resource="https://raw.githubusercontent.com/TheWorldAvatar/ontovertopping/refs/heads/main/OntOvertopping.owl#InputParameter"/>
        <rdfs:comment>An object property that links an overtopping forecast model to the input parameters it requires for prediction.</rdfs:comment>
        <rdfs:isDefinedBy rdf:resource="https://raw.githubusercontent.com/TheWorldAvatar/ontovertopping/refs/heads/main/OntOvertopping.owl"/>
        <rdfs:label>hasInputParameter</rdfs:label>
    </owl:ObjectProperty>
    


    <!-- https://raw.githubusercontent.com/TheWorldAvatar/ontovertopping/refs/heads/main/OntOvertopping.owl#hasOutputParameter -->


    <owl:ObjectProperty rdf:about="https://raw.githubusercontent.com/TheWorldAvatar/ontovertopping/refs/heads/main/OntOvertopping.owl#hasOutputParameter">
        <rdfs:domain rdf:resource="https://raw.githubusercontent.com/TheWorldAvatar/ontovertopping/refs/heads/main/OntOvertopping.owl#OvertoppingForecastModel"/>
        <rdfs:range rdf:resource="https://raw.githubusercontent.com/TheWorldAvatar/ontovertopping/refs/heads/main/OntOvertopping.owl#OutputParameter"/>
        <rdfs:comment>An object property that links an overtopping forecast model to the output parameters it predicts.</rdfs:comment>
        <rdfs:isDefinedBy rdf:resource="https://raw.githubusercontent.com/TheWorldAvatar/ontovertopping/refs/heads/main/OntOvertopping.owl"/>
        <rdfs:label>hasOutputParameter</rdfs:label>
    </owl:ObjectProperty>
    


    <!-- https://raw.githubusercontent.com/TheWorldAvatar/ontovertopping/refs/heads/main/OntOvertopping.owl#hasOvertoppingInputParameter -->


    <owl:ObjectProperty rdf:about="https://raw.githubusercontent.com/TheWorldAvatar/ontovertopping/refs/heads/main/OntOvertopping.owl#hasOvertoppingInputParameter">
        <rdfs:subPropertyOf rdf:resource="https://raw.githubusercontent.com/TheWorldAvatar/ontovertopping/refs/heads/main/OntOvertopping.owl#hasInputParameter"/>
        <rdfs:domain rdf:resource="https://raw.githubusercontent.com/TheWorldAvatar/ontovertopping/refs/heads/main/OntOvertopping.owl#NN_Overtopping2"/>
        <rdfs:range>
            <owl:Class>
                <owl:unionOf rdf:parseType="Collection">
                    <rdf:Description rdf:about="https://raw.githubusercontent.com/TheWorldAvatar/ontovertopping/refs/heads/main/OntOvertopping.owl#AngleOfDownSlope"/>
                    <rdf:Description rdf:about="https://raw.githubusercontent.com/TheWorldAvatar/ontovertopping/refs/heads/main/OntOvertopping.owl#AngleOfUpperSlope"/>
                    <rdf:Description rdf:about="https://raw.githubusercontent.com/TheWorldAvatar/ontovertopping/refs/heads/main/OntOvertopping.owl#AngleOfWaveAttack"/>
                    <rdf:Description rdf:about="https://raw.githubusercontent.com/TheWorldAvatar/ontovertopping/refs/heads/main/OntOvertopping.owl#ArmourFreeboardRelativeToSWL"/>
                    <rdf:Description rdf:about="https://raw.githubusercontent.com/TheWorldAvatar/ontovertopping/refs/heads/main/OntOvertopping.owl#ArmourWidth"/>
                    <rdf:Description rdf:about="https://raw.githubusercontent.com/TheWorldAvatar/ontovertopping/refs/heads/main/OntOvertopping.owl#BermSlope"/>
                    <rdf:Description rdf:about="https://raw.githubusercontent.com/TheWorldAvatar/ontovertopping/refs/heads/main/OntOvertopping.owl#BermWidth"/>
                    <rdf:Description rdf:about="https://raw.githubusercontent.com/TheWorldAvatar/ontovertopping/refs/heads/main/OntOvertopping.owl#CrestFreeboardRelativeToSWL"/>
                    <rdf:Description rdf:about="https://raw.githubusercontent.com/TheWorldAvatar/ontovertopping/refs/heads/main/OntOvertopping.owl#RoughnessCoefficient"/>
                    <rdf:Description rdf:about="https://raw.githubusercontent.com/TheWorldAvatar/ontovertopping/refs/heads/main/OntOvertopping.owl#SignificantWaveHeight"/>
                    <rdf:Description rdf:about="https://raw.githubusercontent.com/TheWorldAvatar/ontovertopping/refs/heads/main/OntOvertopping.owl#WaterDepthAtToeOfBreakwater"/>
                    <rdf:Description rdf:about="https://raw.githubusercontent.com/TheWorldAvatar/ontovertopping/refs/heads/main/OntOvertopping.owl#WaterDepthInFrontOfStructure"/>
                    <rdf:Description rdf:about="https://raw.githubusercontent.com/TheWorldAvatar/ontovertopping/refs/heads/main/OntOvertopping.owl#WaterDepthOnBerm"/>
                    <rdf:Description rdf:about="https://raw.githubusercontent.com/TheWorldAvatar/ontovertopping/refs/heads/main/OntOvertopping.owl#WavePeriod"/>
                    <rdf:Description rdf:about="https://raw.githubusercontent.com/TheWorldAvatar/ontovertopping/refs/heads/main/OntOvertopping.owl#WidthOfToe"/>
                </owl:unionOf>
            </owl:Class>
        </rdfs:range>
        <rdfs:comment>An input parameter required for the NN_Overtopping2 model.</rdfs:comment>
        <rdfs:label>hasOvertoppingInputParameter</rdfs:label>
    </owl:ObjectProperty>
    


    <!-- https://raw.githubusercontent.com/TheWorldAvatar/ontovertopping/refs/heads/main/OntOvertopping.owl#hasOvertoppingOutputParameter -->


    <owl:ObjectProperty rdf:about="https://raw.githubusercontent.com/TheWorldAvatar/ontovertopping/refs/heads/main/OntOvertopping.owl#hasOvertoppingOutputParameter">
        <rdfs:subPropertyOf rdf:resource="https://raw.githubusercontent.com/TheWorldAvatar/ontovertopping/refs/heads/main/OntOvertopping.owl#hasOutputParameter"/>
        <rdfs:domain rdf:resource="https://raw.githubusercontent.com/TheWorldAvatar/ontovertopping/refs/heads/main/OntOvertopping.owl#NN_Overtopping2"/>
        <rdfs:range rdf:resource="https://raw.githubusercontent.com/TheWorldAvatar/ontovertopping/refs/heads/main/OntOvertopping.owl#MeanOvertoppingDischarge"/>
        <rdfs:comment>An output parameter representing the </rdfs:comment>
        <rdfs:label>hasOvertoppingOutputParameter</rdfs:label>
    </owl:ObjectProperty>
    


    <!-- https://raw.githubusercontent.com/TheWorldAvatar/ontovertopping/refs/heads/main/OntOvertopping.owl#hasPart -->


    <owl:ObjectProperty rdf:about="https://raw.githubusercontent.com/TheWorldAvatar/ontovertopping/refs/heads/main/OntOvertopping.owl#hasPart">
        <rdfs:domain rdf:resource="https://raw.githubusercontent.com/TheWorldAvatar/ontovertopping/refs/heads/main/OntOvertopping.owl#CoastalDefenceStructure"/>
        <rdfs:range rdf:resource="https://raw.githubusercontent.com/TheWorldAvatar/ontovertopping/refs/heads/main/OntOvertopping.owl#CrestWall"/>
        <rdfs:comment>An object property that relates a CoastalDefenceStructure to one of its structural components, such as a CrestWall.</rdfs:comment>
        <rdfs:label>hasPart</rdfs:label>
    </owl:ObjectProperty>
    


    <!-- https://raw.githubusercontent.com/TheWorldAvatar/ontovertopping/refs/heads/main/OntOvertopping.owl#hasWaveCondition -->


    <owl:ObjectProperty rdf:about="https://raw.githubusercontent.com/TheWorldAvatar/ontovertopping/refs/heads/main/OntOvertopping.owl#hasWaveCondition">
        <rdfs:domain rdf:resource="https://raw.githubusercontent.com/TheWorldAvatar/ontovertopping/refs/heads/main/OntOvertopping.owl#Wave"/>
        <rdfs:range rdf:resource="https://raw.githubusercontent.com/TheWorldAvatar/ontovertopping/refs/heads/main/OntOvertopping.owl#WaveCondition"/>
        <rdfs:comment>Relates a wave to its associated WaveCondition (e.g., height, period, angle and direction).</rdfs:comment>
        <rdfs:isDefinedBy rdf:resource="https://raw.githubusercontent.com/TheWorldAvatar/ontovertopping/refs/heads/main/OntOvertopping.owl"/>
        <rdfs:label>hasWaveCondition</rdfs:label>
    </owl:ObjectProperty>
    


    <!-- https://raw.githubusercontent.com/TheWorldAvatar/ontovertopping/refs/heads/main/OntOvertopping.owl#isMeasuredAgainst -->


    <owl:ObjectProperty rdf:about="https://raw.githubusercontent.com/TheWorldAvatar/ontovertopping/refs/heads/main/OntOvertopping.owl#isMeasuredAgainst">
        <rdfs:domain rdf:resource="https://raw.githubusercontent.com/TheWorldAvatar/ontovertopping/refs/heads/main/OntOvertopping.owl#AngleOfWaveAttack"/>
        <rdfs:range rdf:resource="https://raw.githubusercontent.com/TheWorldAvatar/ontovertopping/refs/heads/main/OntOvertopping.owl#CrestWall"/>
        <rdfs:comment>Relates the AngleOfWaveAttack to the CrestWall that serves as the reference structure for the angle measurement.</rdfs:comment>
        <rdfs:isDefinedBy rdf:resource="https://raw.githubusercontent.com/TheWorldAvatar/ontovertopping/refs/heads/main/OntOvertopping.owl"/>
        <rdfs:label>isMeasuredAgainst</rdfs:label>
    </owl:ObjectProperty>
    


    <!-- https://raw.githubusercontent.com/TheWorldAvatar/ontovertopping/refs/heads/main/OntOvertopping.owl#managesForecastOf -->


    <owl:ObjectProperty rdf:about="https://raw.githubusercontent.com/TheWorldAvatar/ontovertopping/refs/heads/main/OntOvertopping.owl#managesForecastOf">
        <rdfs:domain rdf:resource="https://raw.githubusercontent.com/TheWorldAvatar/ontovertopping/refs/heads/main/OntOvertopping.owl#OvertoppingForecast"/>
        <rdfs:range rdf:resource="https://raw.githubusercontent.com/TheWorldAvatar/ontovertopping/refs/heads/main/OntOvertopping.owl#Overtopping"/>
        <rdfs:comment>An object property that links an overtopping forecast to the actual overtopping event it aims to predict or manage.</rdfs:comment>
        <rdfs:isDefinedBy rdf:resource="https://raw.githubusercontent.com/TheWorldAvatar/ontovertopping/refs/heads/main/OntOvertopping.owl"/>
        <rdfs:label>managesForecastOf</rdfs:label>
    </owl:ObjectProperty>
    


    <!-- https://raw.githubusercontent.com/TheWorldAvatar/ontovertopping/refs/heads/main/OntOvertopping.owl#measuredAt -->


    <owl:ObjectProperty rdf:about="https://raw.githubusercontent.com/TheWorldAvatar/ontovertopping/refs/heads/main/OntOvertopping.owl#measuredAt">
        <rdfs:domain rdf:resource="https://raw.githubusercontent.com/TheWorldAvatar/ontovertopping/refs/heads/main/OntOvertopping.owl#MeanOvertoppingDischarge"/>
        <rdfs:range rdf:resource="https://raw.githubusercontent.com/TheWorldAvatar/ontovertopping/refs/heads/main/OntOvertopping.owl#CrestWall"/>
        <rdfs:comment>An object property relating an instance of OvertoppingDischarge to the physical structure, e.g., a breakwater or crest wall, where the overtopping discharge occurs and is measured.</rdfs:comment>
        <rdfs:label>MeanOvertoppingDischarge</rdfs:label>
    </owl:ObjectProperty>
    


    <!-- 
    ///////////////////////////////////////////////////////////////////////////////////////
    //
    // Data properties
    //
    ///////////////////////////////////////////////////////////////////////////////////////
     -->


    


    <!-- http://www.ontology-of-units-of-measure.org/resource/om-2/hasNumericalValue -->


    <owl:DatatypeProperty rdf:about="http://www.ontology-of-units-of-measure.org/resource/om-2/hasNumericalValue">
        <rdfs:domain rdf:resource="http://www.ontology-of-units-of-measure.org/resource/om-2/Measure"/>
        <rdfs:range rdf:resource="http://www.w3.org/2001/XMLSchema#float"/>
        <rdfs:comment>The numerical value of a measured quantity.</rdfs:comment>
        <rdfs:isDefinedBy rdf:resource="http://www.ontology-of-units-of-measure.org/resource/om-2"/>
        <rdfs:label>hasNumericalValue</rdfs:label>
    </owl:DatatypeProperty>
    


    <!-- 
    ///////////////////////////////////////////////////////////////////////////////////////
    //
    // Classes
    //
    ///////////////////////////////////////////////////////////////////////////////////////
     -->


    


    <!-- http://www.ontology-of-units-of-measure.org/resource/om-2/Measure -->


    <owl:Class rdf:about="http://www.ontology-of-units-of-measure.org/resource/om-2/Measure"/>
    


    <!-- http://www.ontology-of-units-of-measure.org/resource/om-2/Quantity -->


    <owl:Class rdf:about="http://www.ontology-of-units-of-measure.org/resource/om-2/Quantity"/>
    


    <!-- http://www.ontology-of-units-of-measure.org/resource/om-2/Unit -->


    <owl:Class rdf:about="http://www.ontology-of-units-of-measure.org/resource/om-2/Unit"/>
    


    <!-- https://raw.githubusercontent.com/TheWorldAvatar/ontovertopping/refs/heads/main/OntOvertopping.owl#AngleOfDownSlope -->


    <owl:Class rdf:about="https://raw.githubusercontent.com/TheWorldAvatar/ontovertopping/refs/heads/main/OntOvertopping.owl#AngleOfDownSlope">
        <rdfs:subClassOf rdf:resource="https://raw.githubusercontent.com/TheWorldAvatar/ontovertopping/refs/heads/main/OntOvertopping.owl#InputParameter"/>
        <rdfs:comment>The inclination angle of the slope located just above and adjacent to the base (toe) of a breakwater.</rdfs:comment>
        <rdfs:isDefinedBy rdf:resource="https://raw.githubusercontent.com/TheWorldAvatar/ontovertopping/refs/heads/main/OntOvertopping.owl"/>
        <rdfs:label>AngleOfDownSlope</rdfs:label>
    </owl:Class>
    


    <!-- https://raw.githubusercontent.com/TheWorldAvatar/ontovertopping/refs/heads/main/OntOvertopping.owl#AngleOfUpperSlope -->


    <owl:Class rdf:about="https://raw.githubusercontent.com/TheWorldAvatar/ontovertopping/refs/heads/main/OntOvertopping.owl#AngleOfUpperSlope">
        <rdfs:subClassOf rdf:resource="https://raw.githubusercontent.com/TheWorldAvatar/ontovertopping/refs/heads/main/OntOvertopping.owl#InputParameter"/>
        <rdfs:comment>The inclination angle of the slope located just below and adjacent to the armour of a breakwater.</rdfs:comment>
        <rdfs:isDefinedBy rdf:resource="https://raw.githubusercontent.com/TheWorldAvatar/ontovertopping/refs/heads/main/OntOvertopping.owl"/>
        <rdfs:label>AngleOfUpperSlope</rdfs:label>
    </owl:Class>
    


    <!-- https://raw.githubusercontent.com/TheWorldAvatar/ontovertopping/refs/heads/main/OntOvertopping.owl#AngleOfWaveAttack -->


    <owl:Class rdf:about="https://raw.githubusercontent.com/TheWorldAvatar/ontovertopping/refs/heads/main/OntOvertopping.owl#AngleOfWaveAttack">
        <rdfs:subClassOf rdf:resource="https://raw.githubusercontent.com/TheWorldAvatar/ontovertopping/refs/heads/main/OntOvertopping.owl#InputParameter"/>
        <rdfs:comment>The angle between the normal to the coastal or breakwater structure and the direction of the incident wave approach.</rdfs:comment>
        <rdfs:isDefinedBy rdf:resource="https://raw.githubusercontent.com/TheWorldAvatar/ontovertopping/refs/heads/main/OntOvertopping.owl"/>
        <rdfs:label>AngleOfWaveAttack</rdfs:label>
    </owl:Class>
    


    <!-- https://raw.githubusercontent.com/TheWorldAvatar/ontovertopping/refs/heads/main/OntOvertopping.owl#ArmourFreeboardRelativeToSWL -->


    <owl:Class rdf:about="https://raw.githubusercontent.com/TheWorldAvatar/ontovertopping/refs/heads/main/OntOvertopping.owl#ArmourFreeboardRelativeToSWL">
        <rdfs:subClassOf rdf:resource="https://raw.githubusercontent.com/TheWorldAvatar/ontovertopping/refs/heads/main/OntOvertopping.owl#InputParameter"/>
        <rdfs:comment>The vertical distance between the crest of the armour layer of a breakwater and the still water level (SWL).</rdfs:comment>
        <rdfs:isDefinedBy rdf:resource="https://raw.githubusercontent.com/TheWorldAvatar/ontovertopping/refs/heads/main/OntOvertopping.owl"/>
        <rdfs:label>ArmourFreeboardRelativeToSWL</rdfs:label>
    </owl:Class>
    


    <!-- https://raw.githubusercontent.com/TheWorldAvatar/ontovertopping/refs/heads/main/OntOvertopping.owl#ArmourWidth -->


    <owl:Class rdf:about="https://raw.githubusercontent.com/TheWorldAvatar/ontovertopping/refs/heads/main/OntOvertopping.owl#ArmourWidth">
        <rdfs:subClassOf rdf:resource="https://raw.githubusercontent.com/TheWorldAvatar/ontovertopping/refs/heads/main/OntOvertopping.owl#InputParameter"/>
        <rdfs:comment>The horizontal thickness of the armour layer on a breakwater.</rdfs:comment>
        <rdfs:isDefinedBy rdf:resource="https://raw.githubusercontent.com/TheWorldAvatar/ontovertopping/refs/heads/main/OntOvertopping.owl"/>
        <rdfs:label>ArmourWidth</rdfs:label>
    </owl:Class>
    


    <!-- https://raw.githubusercontent.com/TheWorldAvatar/ontovertopping/refs/heads/main/OntOvertopping.owl#BermSlope -->


    <owl:Class rdf:about="https://raw.githubusercontent.com/TheWorldAvatar/ontovertopping/refs/heads/main/OntOvertopping.owl#BermSlope">
        <rdfs:subClassOf rdf:resource="https://raw.githubusercontent.com/TheWorldAvatar/ontovertopping/refs/heads/main/OntOvertopping.owl#InputParameter"/>
        <rdfs:comment>The inclination angle of the berm surface, typically measured relative to the horizontal plane.</rdfs:comment>
        <rdfs:isDefinedBy rdf:resource="https://raw.githubusercontent.com/TheWorldAvatar/ontovertopping/refs/heads/main/OntOvertopping.owl"/>
        <rdfs:label>BermSlope</rdfs:label>
    </owl:Class>
    


    <!-- https://raw.githubusercontent.com/TheWorldAvatar/ontovertopping/refs/heads/main/OntOvertopping.owl#BermWidth -->


    <owl:Class rdf:about="https://raw.githubusercontent.com/TheWorldAvatar/ontovertopping/refs/heads/main/OntOvertopping.owl#BermWidth">
        <rdfs:subClassOf rdf:resource="https://raw.githubusercontent.com/TheWorldAvatar/ontovertopping/refs/heads/main/OntOvertopping.owl#InputParameter"/>
        <rdfs:comment>The horizontal distance across the gently sloping section of a breakwater, typically located between the down slope and the upper slope.</rdfs:comment>
        <rdfs:isDefinedBy rdf:resource="https://raw.githubusercontent.com/TheWorldAvatar/ontovertopping/refs/heads/main/OntOvertopping.owl"/>
        <rdfs:label>BermWidth</rdfs:label>
    </owl:Class>
    


    <!-- https://raw.githubusercontent.com/TheWorldAvatar/ontovertopping/refs/heads/main/OntOvertopping.owl#CoastalDefenceStructure -->


    <owl:Class rdf:about="https://raw.githubusercontent.com/TheWorldAvatar/ontovertopping/refs/heads/main/OntOvertopping.owl#CoastalDefenceStructure">
        <rdfs:comment>A structure built in coastal areas to protect entities such as ports, roads, railways, and their associated services from the impacts of waves, tides, and flooding.</rdfs:comment>
        <rdfs:isDefinedBy rdf:resource="https://raw.githubusercontent.com/TheWorldAvatar/ontovertopping/refs/heads/main/OntOvertopping.owl"/>
        <rdfs:label>CoastalDefenceStructure</rdfs:label>
    </owl:Class>
    


    <!-- https://raw.githubusercontent.com/TheWorldAvatar/ontovertopping/refs/heads/main/OntOvertopping.owl#CrestFreeboardRelativeToSWL -->


    <owl:Class rdf:about="https://raw.githubusercontent.com/TheWorldAvatar/ontovertopping/refs/heads/main/OntOvertopping.owl#CrestFreeboardRelativeToSWL">
        <rdfs:subClassOf rdf:resource="https://raw.githubusercontent.com/TheWorldAvatar/ontovertopping/refs/heads/main/OntOvertopping.owl#InputParameter"/>
        <rdfs:comment>The vertical distance between the still water level (SWL) and the crest of a breakwater.</rdfs:comment>
        <rdfs:isDefinedBy rdf:resource="https://raw.githubusercontent.com/TheWorldAvatar/ontovertopping/refs/heads/main/OntOvertopping.owl"/>
        <rdfs:label>CrestFreeboardRelativeToSWL</rdfs:label>
    </owl:Class>
    


    <!-- https://raw.githubusercontent.com/TheWorldAvatar/ontovertopping/refs/heads/main/OntOvertopping.owl#CrestWall -->


    <owl:Class rdf:about="https://raw.githubusercontent.com/TheWorldAvatar/ontovertopping/refs/heads/main/OntOvertopping.owl#CrestWall">
        <rdfs:comment>A wall constructed landward of the crest, functioning as part of a breakwater structure.</rdfs:comment>
        <rdfs:isDefinedBy rdf:resource="https://raw.githubusercontent.com/TheWorldAvatar/ontovertopping/refs/heads/main/OntOvertopping.owl"/>
        <rdfs:label>CrestWall</rdfs:label>
    </owl:Class>
    


    <!-- https://raw.githubusercontent.com/TheWorldAvatar/ontovertopping/refs/heads/main/OntOvertopping.owl#DerivedQuantity -->


    <owl:Class rdf:about="https://raw.githubusercontent.com/TheWorldAvatar/ontovertopping/refs/heads/main/OntOvertopping.owl#DerivedQuantity">
        <rdfs:subClassOf rdf:resource="http://www.ontology-of-units-of-measure.org/resource/om-2/Quantity"/>
        <rdfs:comment>A quantity computed from a combination of other input parameters or measurements, rather than being directly observed.</rdfs:comment>
        <rdfs:isDefinedBy rdf:resource="https://raw.githubusercontent.com/TheWorldAvatar/ontovertopping/refs/heads/main/OntOvertopping.owl"/>
        <rdfs:label>DerivedQuantity</rdfs:label>
    </owl:Class>
    


    <!-- https://raw.githubusercontent.com/TheWorldAvatar/ontovertopping/refs/heads/main/OntOvertopping.owl#InputParameter -->


    <owl:Class rdf:about="https://raw.githubusercontent.com/TheWorldAvatar/ontovertopping/refs/heads/main/OntOvertopping.owl#InputParameter">
        <rdfs:subClassOf rdf:resource="http://www.ontology-of-units-of-measure.org/resource/om-2/Quantity"/>
        <rdfs:comment>A parameter provided as input to a forecast model.</rdfs:comment>
        <rdfs:isDefinedBy rdf:resource="https://raw.githubusercontent.com/TheWorldAvatar/ontovertopping/refs/heads/main/OntOvertopping.owl"/>
        <rdfs:label>InputParameter</rdfs:label>
    </owl:Class>
    


    <!-- https://raw.githubusercontent.com/TheWorldAvatar/ontovertopping/refs/heads/main/OntOvertopping.owl#MeanOvertoppingDischarge -->


    <owl:Class rdf:about="https://raw.githubusercontent.com/TheWorldAvatar/ontovertopping/refs/heads/main/OntOvertopping.owl#MeanOvertoppingDischarge">
        <rdfs:subClassOf rdf:resource="https://raw.githubusercontent.com/TheWorldAvatar/ontovertopping/refs/heads/main/OntOvertopping.owl#DerivedQuantity"/>
        <rdfs:subClassOf rdf:resource="https://raw.githubusercontent.com/TheWorldAvatar/ontovertopping/refs/heads/main/OntOvertopping.owl#OutputParameter"/>
        <rdfs:comment>A derived quantity indicating the volume of water per unit time that flows over a breakwater or crest wall due to wave action.</rdfs:comment>
        <rdfs:isDefinedBy rdf:resource="https://raw.githubusercontent.com/TheWorldAvatar/ontovertopping/refs/heads/main/OntOvertopping.owl"/>
        <rdfs:label>MeanOvertoppingDischarge</rdfs:label>
    </owl:Class>
    


    <!-- https://raw.githubusercontent.com/TheWorldAvatar/ontovertopping/refs/heads/main/OntOvertopping.owl#NN_Overtopping2 -->


    <owl:Class rdf:about="https://raw.githubusercontent.com/TheWorldAvatar/ontovertopping/refs/heads/main/OntOvertopping.owl#NN_Overtopping2">
        <rdfs:subClassOf rdf:resource="https://raw.githubusercontent.com/TheWorldAvatar/ontovertopping/refs/heads/main/OntOvertopping.owl#OvertoppingForecastModel"/>
        <rdfs:comment>A machine learning-based model, specifically a neural network model, used to predict the mean wave overtopping discharge per unit crest length.</rdfs:comment>
        <rdfs:isDefinedBy rdf:resource="https://raw.githubusercontent.com/TheWorldAvatar/ontovertopping/refs/heads/main/OntOvertopping.owl"/>
        <rdfs:label>NN_Overtopping2</rdfs:label>
    </owl:Class>
    


    <!-- https://raw.githubusercontent.com/TheWorldAvatar/ontovertopping/refs/heads/main/OntOvertopping.owl#OutputParameter -->


    <owl:Class rdf:about="https://raw.githubusercontent.com/TheWorldAvatar/ontovertopping/refs/heads/main/OntOvertopping.owl#OutputParameter">
        <rdfs:subClassOf rdf:resource="http://www.ontology-of-units-of-measure.org/resource/om-2/Quantity"/>
        <rdfs:comment>A parameter generated as output by a forecast model.</rdfs:comment>
        <rdfs:isDefinedBy rdf:resource="https://raw.githubusercontent.com/TheWorldAvatar/ontovertopping/refs/heads/main/OntOvertopping.owl"/>
        <rdfs:label>OutputParameter</rdfs:label>
    </owl:Class>
    


    <!-- https://raw.githubusercontent.com/TheWorldAvatar/ontovertopping/refs/heads/main/OntOvertopping.owl#Overtopping -->


    <owl:Class rdf:about="https://raw.githubusercontent.com/TheWorldAvatar/ontovertopping/refs/heads/main/OntOvertopping.owl#Overtopping">
        <rdfs:comment>The physical phenomenon of water rising and flowing over a flood defence structure, e.g., breakwater, dam, wall or dike.</rdfs:comment>
        <rdfs:isDefinedBy rdf:resource="https://raw.githubusercontent.com/TheWorldAvatar/ontovertopping/refs/heads/main/OntOvertopping.owl"/>
        <rdfs:label>Overtopping</rdfs:label>
    </owl:Class>
    


    <!-- https://raw.githubusercontent.com/TheWorldAvatar/ontovertopping/refs/heads/main/OntOvertopping.owl#OvertoppingForecast -->


    <owl:Class rdf:about="https://raw.githubusercontent.com/TheWorldAvatar/ontovertopping/refs/heads/main/OntOvertopping.owl#OvertoppingForecast">
        <rdfs:comment>A prediction of potential overtopping, which may be caused by wave action or a rise in water level.</rdfs:comment>
        <rdfs:isDefinedBy rdf:resource="https://raw.githubusercontent.com/TheWorldAvatar/ontovertopping/refs/heads/main/OntOvertopping.owl"/>
        <rdfs:label>OvertoppingForecast</rdfs:label>
    </owl:Class>
    


    <!-- https://raw.githubusercontent.com/TheWorldAvatar/ontovertopping/refs/heads/main/OntOvertopping.owl#OvertoppingForecastModel -->


    <owl:Class rdf:about="https://raw.githubusercontent.com/TheWorldAvatar/ontovertopping/refs/heads/main/OntOvertopping.owl#OvertoppingForecastModel">
        <rdfs:comment>A computation model, either machine learning-based or rule-based, designed to predict overtopping events.</rdfs:comment>
        <rdfs:isDefinedBy rdf:resource="https://raw.githubusercontent.com/TheWorldAvatar/ontovertopping/refs/heads/main/OntOvertopping.owl"/>
        <rdfs:label>OvertoppingForecastModel</rdfs:label>
    </owl:Class>
    


    <!-- https://raw.githubusercontent.com/TheWorldAvatar/ontovertopping/refs/heads/main/OntOvertopping.owl#RoughnessCoefficient -->


    <owl:Class rdf:about="https://raw.githubusercontent.com/TheWorldAvatar/ontovertopping/refs/heads/main/OntOvertopping.owl#RoughnessCoefficient">
        <rdfs:subClassOf rdf:resource="https://raw.githubusercontent.com/TheWorldAvatar/ontovertopping/refs/heads/main/OntOvertopping.owl#InputParameter"/>
        <rdfs:comment>A coefficient representing the influence of surface texture and structural features of a breakwater on the dissipation of wave energy.</rdfs:comment>
        <rdfs:isDefinedBy rdf:resource="https://raw.githubusercontent.com/TheWorldAvatar/ontovertopping/refs/heads/main/OntOvertopping.owl"/>
        <rdfs:label>RoughnessCoefficient</rdfs:label>
    </owl:Class>
    


    <!-- https://raw.githubusercontent.com/TheWorldAvatar/ontovertopping/refs/heads/main/OntOvertopping.owl#SignificantWaveHeight -->


    <owl:Class rdf:about="https://raw.githubusercontent.com/TheWorldAvatar/ontovertopping/refs/heads/main/OntOvertopping.owl#SignificantWaveHeight">
        <rdfs:subClassOf rdf:resource="https://raw.githubusercontent.com/TheWorldAvatar/ontovertopping/refs/heads/main/OntOvertopping.owl#InputParameter"/>
        <rdfs:comment>The vertical distance between the base (toe) of a breakwater and the average height of the most energetic portion of the wave spectrum attacking the breakwater.</rdfs:comment>
        <rdfs:isDefinedBy rdf:resource="https://raw.githubusercontent.com/TheWorldAvatar/ontovertopping/refs/heads/main/OntOvertopping.owl"/>
        <rdfs:label>SignificantWaveHeight</rdfs:label>
    </owl:Class>
    


    <!-- https://raw.githubusercontent.com/TheWorldAvatar/ontovertopping/refs/heads/main/OntOvertopping.owl#WaterDepthAtToeOfBreakwater -->


    <owl:Class rdf:about="https://raw.githubusercontent.com/TheWorldAvatar/ontovertopping/refs/heads/main/OntOvertopping.owl#WaterDepthAtToeOfBreakwater">
        <rdfs:subClassOf rdf:resource="https://raw.githubusercontent.com/TheWorldAvatar/ontovertopping/refs/heads/main/OntOvertopping.owl#InputParameter"/>
        <rdfs:subClassOf rdf:resource="https://raw.githubusercontent.com/TheWorldAvatar/ontovertopping/refs/heads/main/OntOvertopping.owl#WaveCondition"/>
        <rdfs:comment>The vertical distance between the still water level (i.e., the water surface under calm conditions) and the seabed at the toe (base) of a breakwater.</rdfs:comment>
        <rdfs:isDefinedBy rdf:resource="https://raw.githubusercontent.com/TheWorldAvatar/ontovertopping/refs/heads/main/OntOvertopping.owl"/>
        <rdfs:label>WaterDepthAtToeOfBreakwater</rdfs:label>
    </owl:Class>
    


    <!-- https://raw.githubusercontent.com/TheWorldAvatar/ontovertopping/refs/heads/main/OntOvertopping.owl#WaterDepthInFrontOfStructure -->


    <owl:Class rdf:about="https://raw.githubusercontent.com/TheWorldAvatar/ontovertopping/refs/heads/main/OntOvertopping.owl#WaterDepthInFrontOfStructure">
        <rdfs:subClassOf rdf:resource="https://raw.githubusercontent.com/TheWorldAvatar/ontovertopping/refs/heads/main/OntOvertopping.owl#InputParameter"/>
        <rdfs:comment>The vertical distance between the base (toe) of a breakwater and the still water level (SWL) in front of the breakwater.</rdfs:comment>
        <rdfs:isDefinedBy rdf:resource="https://raw.githubusercontent.com/TheWorldAvatar/ontovertopping/refs/heads/main/OntOvertopping.owl"/>
        <rdfs:label>WaterDepthInFrontOfStructure</rdfs:label>
    </owl:Class>
    


    <!-- https://raw.githubusercontent.com/TheWorldAvatar/ontovertopping/refs/heads/main/OntOvertopping.owl#WaterDepthOnBerm -->


    <owl:Class rdf:about="https://raw.githubusercontent.com/TheWorldAvatar/ontovertopping/refs/heads/main/OntOvertopping.owl#WaterDepthOnBerm">
        <rdfs:subClassOf rdf:resource="https://raw.githubusercontent.com/TheWorldAvatar/ontovertopping/refs/heads/main/OntOvertopping.owl#InputParameter"/>
        <rdfs:comment>The vertical distance between the lowest elevation point of the berm and the still water level (SWL) in front of a breakwater.</rdfs:comment>
        <rdfs:isDefinedBy rdf:resource="https://raw.githubusercontent.com/TheWorldAvatar/ontovertopping/refs/heads/main/OntOvertopping.owl"/>
        <rdfs:label>WaterDepthOnBerm</rdfs:label>
    </owl:Class>
    


    <!-- https://raw.githubusercontent.com/TheWorldAvatar/ontovertopping/refs/heads/main/OntOvertopping.owl#Wave -->


    <owl:Class rdf:about="https://raw.githubusercontent.com/TheWorldAvatar/ontovertopping/refs/heads/main/OntOvertopping.owl#Wave">
        <rdfs:comment>One of a series of ridges that moves across the surface of a liquid (especially across a large body of water) [EN Wordnet]</rdfs:comment>
        <rdfs:isDefinedBy rdf:resource="https://raw.githubusercontent.com/TheWorldAvatar/ontovertopping/refs/heads/main/OntOvertopping.owl"/>
        <rdfs:label>Wave</rdfs:label>
    </owl:Class>
    


    <!-- https://raw.githubusercontent.com/TheWorldAvatar/ontovertopping/refs/heads/main/OntOvertopping.owl#WaveAngle -->


    <owl:Class rdf:about="https://raw.githubusercontent.com/TheWorldAvatar/ontovertopping/refs/heads/main/OntOvertopping.owl#WaveAngle">
        <rdfs:subClassOf rdf:resource="https://raw.githubusercontent.com/TheWorldAvatar/ontovertopping/refs/heads/main/OntOvertopping.owl#WaveCondition"/>
        <rdfs:comment>The angle between the incoming wave direction and a specific structure or shoreline orientation, usually measured relative to the normal (perpendicular) to that structure.</rdfs:comment>
        <rdfs:isDefinedBy rdf:resource="https://raw.githubusercontent.com/TheWorldAvatar/ontovertopping/refs/heads/main/OntOvertopping.owl"/>
        <rdfs:label>WaveAngle</rdfs:label>
    </owl:Class>
    


    <!-- https://raw.githubusercontent.com/TheWorldAvatar/ontovertopping/refs/heads/main/OntOvertopping.owl#WaveCondition -->


    <owl:Class rdf:about="https://raw.githubusercontent.com/TheWorldAvatar/ontovertopping/refs/heads/main/OntOvertopping.owl#WaveCondition">
        <rdfs:subClassOf rdf:resource="http://www.ontology-of-units-of-measure.org/resource/om-2/Quantity"/>
        <rdfs:comment>The characteristics of a wave, such as wave height, period, angle and direction.</rdfs:comment>
        <rdfs:isDefinedBy rdf:resource="https://raw.githubusercontent.com/TheWorldAvatar/ontovertopping/refs/heads/main/OntOvertopping.owl"/>
        <rdfs:label>WaveCondition</rdfs:label>
    </owl:Class>
    


    <!-- https://raw.githubusercontent.com/TheWorldAvatar/ontovertopping/refs/heads/main/OntOvertopping.owl#WaveDirection -->


    <owl:Class rdf:about="https://raw.githubusercontent.com/TheWorldAvatar/ontovertopping/refs/heads/main/OntOvertopping.owl#WaveDirection">
        <rdfs:subClassOf rdf:resource="https://raw.githubusercontent.com/TheWorldAvatar/ontovertopping/refs/heads/main/OntOvertopping.owl#WaveCondition"/>
        <rdfs:comment>The compass direction from which the waves are coming, typically measured in degrees clockwise from true north (0°–360°).</rdfs:comment>
        <rdfs:isDefinedBy rdf:resource="https://raw.githubusercontent.com/TheWorldAvatar/ontovertopping/refs/heads/main/OntOvertopping.owl"/>
        <rdfs:label>WaveDirection</rdfs:label>
    </owl:Class>
    


    <!-- https://raw.githubusercontent.com/TheWorldAvatar/ontovertopping/refs/heads/main/OntOvertopping.owl#WavePeriod -->


    <owl:Class rdf:about="https://raw.githubusercontent.com/TheWorldAvatar/ontovertopping/refs/heads/main/OntOvertopping.owl#WavePeriod">
        <rdfs:subClassOf rdf:resource="https://raw.githubusercontent.com/TheWorldAvatar/ontovertopping/refs/heads/main/OntOvertopping.owl#InputParameter"/>
        <rdfs:subClassOf rdf:resource="https://raw.githubusercontent.com/TheWorldAvatar/ontovertopping/refs/heads/main/OntOvertopping.owl#WaveCondition"/>
        <rdfs:comment>The time interval between two successive wave crests passing a fixed point, such as a crest wall.</rdfs:comment>
        <rdfs:isDefinedBy rdf:resource="https://raw.githubusercontent.com/TheWorldAvatar/ontovertopping/refs/heads/main/OntOvertopping.owl"/>
        <rdfs:label>WavePeriod</rdfs:label>
    </owl:Class>
    


    <!-- https://raw.githubusercontent.com/TheWorldAvatar/ontovertopping/refs/heads/main/OntOvertopping.owl#WidthOfToe -->


    <owl:Class rdf:about="https://raw.githubusercontent.com/TheWorldAvatar/ontovertopping/refs/heads/main/OntOvertopping.owl#WidthOfToe">
        <rdfs:subClassOf rdf:resource="https://raw.githubusercontent.com/TheWorldAvatar/ontovertopping/refs/heads/main/OntOvertopping.owl#InputParameter"/>
        <rdfs:comment>The horizontal distance across the base (toe) of a breakwater, measured from its landward edge to its seaward edge.</rdfs:comment>
        <rdfs:isDefinedBy rdf:resource="https://raw.githubusercontent.com/TheWorldAvatar/ontovertopping/refs/heads/main/OntOvertopping.owl"/>
        <rdfs:label>WidthOfToe</rdfs:label>
    </owl:Class>
</rdf:RDF>



<!-- Generated by the OWL API (version 5.5.0.2023-01-14T12:41:38Z) https://github.com/owlcs/owlapi/ -->


